Get graphOf to halfway reasonable state prior to radical rework.
In particular, I now think that it's impossible to get the graph
framework to cope with the difference between local and global scopes
and, worse, nested local scopes. So, instead I'll assume one memory
map, and rely on higher levels to translate variable names apart from
one another.

The initialisation of local variables in for- and par- loop iterations
can be explicitly done with assignments that are generated by the
semantics as it executes.

hol/PseudoCPropsScript.sml
@@ -699,46 +699,73 @@ val apply_action_commutes = store_thm(
   rpt (findOptionCases >> simp[]) >> TRY eqNONE_tac >>
   success_case)
 
+val commutes_lemma = prove(
+  ``∀a1 a2 s.
+      ¬(a1 ∼ₜ a2) ∧ a1.iter ≠ a2.iter ⇒
+      apply_action a2 (apply_action a1 s) =
+      apply_action a1 (apply_action a2 s)``,
+  simp[apply_action_commutes]);
+
+val pcg_eval_def = Define`
+  pcg_eval g s = gEVAL apply_action s g
+`;
+
+val pcg_eval_thm = save_thm(
+  "pcg_eval_thm",
+  MATCH_MP gEVAL_thm commutes_lemma
+           |> REWRITE_RULE [GSYM pcg_eval_def]);
+
+val pop_scope_def = Define`
+  pop_scope old nested new =
+    DRESTRICT new (COMPL (FDOM nested)) ⊌ old
+`;
+
 val graphOf_def = tDefine "graphOf" `
 
-  (graphOf i lm m G0 (IfStmt g t e) =
+  (graphOf i lm m (IfStmt g t e) =
      case evalexpr (lm ⊌ m) g of
-       | Bool T => graphOf i lm m G0 t
-       | Bool F => graphOf i lm m G0 e
+       | Bool T => graphOf i lm m t
+       | Bool F => graphOf i lm m e
        | _ => NONE) ∧
 
-  (graphOf i lm0 m0 G0 (ForLoop vnm d body) =
+  (graphOf i lm0 m0 (ForLoop vnm d body) =
      do
        dvs <- dvalues (lm0 ⊌ m0) d;
-       graphOf i lm0 m0 G0 (Seq (MAP (λv. (FEMPTY |+ (vnm,v),body)) dvs))
+       graphOf i lm0 m0 (Seq (MAP (λv. (FEMPTY |+ (vnm,v),body)) dvs))
      od) ∧
 
-  (graphOf i lm0 m0 G0 (Seq cmds) =
+  (graphOf i lm0 m0 (Seq cmds) =
      case cmds of
-       | [] => SOME (lm0, m0, G0)
+       | [] => SOME (lm0, m0, emptyG)
        | (lm,c) :: rest =>
          do
-           (lm', m', G') <- graphOf i (lm ⊌ lm0) m0 G0 c;
-           graphOf (stackInc i) lm0 m' G' (Seq rest)
+           (lm1, m1, G1) <- graphOf i (lm ⊌ lm0) m0 c;
+           lm1' <- SOME (pop_scope lm0 lm lm1);
+           (lm2, m2, G2) <- graphOf (stackInc i) lm1' m1 (Seq rest);
+           SOME(lm2,m2,merge_graph G1 G2)
          od) ∧
 
-  (graphOf i lm0 m0 G0 (ParLoop vnm d body) =
+  (graphOf i lm0 m0 (ParLoop vnm d body) =
      do
        dvs <- dvalues (lm0 ⊌ m0) d;
-       graphOf i lm0 m0 G0 (Par (MAP (λv. (FEMPTY |+ (vnm,v), body)) dvs))
+       graphOf i lm0 m0 (Par (MAP (λv. (FEMPTY |+ (vnm,v), body)) dvs))
      od) ∧
 
-  (graphOf i lm0 m0 G0 (Par cmds) =
+  (graphOf i lm0 m0 (Par cmds) =
      do
-       ps0 <- OPT_SEQUENCE (MAP (λ(lm,c). graphOf i (lm ⊌ lm0) m0 G0 c) cmds);
-       ps <- SOME (GENLIST (λn. ap3 (pushG n) (EL n ps0)) (LENGTH ps0));
-       assert(∀i j. i < j ∧ j < LENGTH ps ⇒
-                    ¬gtouches (SND (SND (EL i ps))) (SND (SND (EL j ps))));
-       SOME(lm0, (@m. ∃lm. eval (lm0, m0, Par cmds) (lm, m, Done)),
-            FOLDR (λ(lm,m,G) aG. merge_graph aG G) (pushG (LENGTH ps0) G0) ps)
+       ps0 <-
+         OPT_SEQUENCE
+           (MAP
+              (λ(lm,c). OPTION_MAP (SND o SND) (graphOf i (lm ⊌ lm0) m0 c))
+              cmds);
+       ps <- SOME (GENLIST (λn. pushG n (EL n ps0)) (LENGTH ps0));
+       assert(∀i j. i < j ∧ j < LENGTH ps ⇒ ¬gtouches (EL i ps) (EL j ps));
+       g <- SOME (FOLDR merge_graph emptyG ps);
+       (lm,m) <- pcg_eval g (SOME(lm0,m0));
+       SOME(lm, m, merge_graph (pushG (LENGTH ps0) G0) g)
      od) ∧
 
-  (graphOf iter lm0 m0 G0 (Assign w ds opn) =
+  (graphOf iter lm0 m0 (Assign w ds opn) =
      do (aname,i_e) <- SOME w;
         i <- (some i. evalexpr (lm0 ⊌ m0) i_e = Int i);
         rds <- getReads (lm0 ⊌ m0) ds;
@@ -748,17 +775,24 @@ val graphOf_def = tDefine "graphOf" `
                      iter := iter |> ;
         rvs <- OPT_SEQUENCE (MAP (evalDexpr (lm0 ⊌ m0)) ds);
         m' <- upd_array m0 aname i (opn rvs);
-        SOME(lm0, m', add_postaction a G0)
+        SOME(lm0, m', a ⊕ emptyG)
      od)
 
 ` (WF_REL_TAC
-     `inv_image (mlt (<) LEX (<)) (λ(i,lm,m,g,s). (loopbag s, stmt_weight s))` >>
+     `inv_image (mlt (<) LEX (<)) (λ(i,lm,m,s). (loopbag s, stmt_weight s))` >>
    simp[WF_mlt1, rich_listTheory.FOLDR_MAP, mlt_loopbag_lemma] >>
    rpt strip_tac
    >- (imp_res_tac MEM_FOLDR_mlt >> pop_assum (qspec_then `SND` mp_tac) >>
        rw[] >> simp[] >> pop_assum kall_tac >> pop_assum mp_tac >>
        map_every qid_spec_tac [`lm`, `c`] >> Induct_on `cmds` >> dsimp[] >>
        rpt strip_tac >> res_tac >> decide_tac))
+
+
+(*val graphOf_correct = store_thm(
+  "graphOf_correct",
+  ``...``
+*)
+
 
 
 val _ = export_theory();
